extend according to the railroad
git-svn-id: https://projects.brucker.ch/hol-testgen/svn/HOL-TestGen/trunk/hol-testgen@11343 3260e6d1-4efc-4170-b0a7-36055960796d

src/compiler/OCL_compiler_generator_dynamic.thy
@@ -1015,7 +1015,7 @@ structure USE_parse = struct
                       | OclTypeBaseUnlimitednatural => OCL.OclTy_base_unlimitednatural
                       | OclTypeBaseReal    => OCL.OclTy_base_real
                       | OclTypeBaseString  => OCL.OclTy_base_string
-                      | OclTypeClassPre s  => OCL.OclTy_class_pre (From.from_binding s)
+                      | OclTypeClassPre s  => OCL.oclTy_class_pre (From.from_binding s)
                       | OclTypeCollectionSet l      => OCL.OclTy_collection (OCL.Ocl_multiplicity_ext ([], NONE, OCL.Set, ()), from_oclty l)
                       | OclTypeCollectionSequence l => OCL.OclTy_collection (OCL.Ocl_multiplicity_ext ([], NONE, OCL.Sequence, ()), from_oclty l)
                       | OclTypePair (s1, s2)        => OCL.OclTy_pair (from_oclty s1, from_oclty s2)
@@ -1081,7 +1081,7 @@ structure USE_parse = struct
    --| colon
    -- use_expression
  (* *)
- val class_def_list = Scan.optional (Parse.$$$ "<" |-- Parse.list1 Parse.binding) []
+ val class_def_list = Scan.repeat (Parse.$$$ "<" |-- Parse.list1 Parse.binding)
  val class_def_attr = Scan.optional (@{keyword "Attributes"}
    |-- Scan.repeat (Parse.binding --| colon -- use_type
                     --| optional Parse.semicolon)) []
@@ -1130,13 +1130,14 @@ end
 
 structure Outer_syntax_Class = struct
   fun make from_expr binding child attribute oper constr =
+    let fun to_pre binding = OCL.OclTyCore_pre (From.from_binding binding) in
     (OCL.Ocl_class_raw_ext
-         ( From.from_binding binding
+         ( OCL.OclTyObj (to_pre binding, map (map to_pre) child)
          , From.from_list (From.from_pair From.from_binding USE_parse.from_oclty) attribute
          , Outer_syntax_Pre_Post.make2 from_expr binding oper
          , Outer_syntax_Inv.make2 from_expr [] binding constr
-         , case child of [] => NONE | [x] => SOME (From.from_binding x)
          , From.from_unit ()))
+    end
 end
 
 local
