src/compiler/core/OCL_compiler_floor1_infra.thy
@@ -109,7 +109,7 @@ definition "print_infra_type_synonym_class_rec = (\<lambda>expr ocl.
                                                            let (tit, body) = print_infra_type_synonym_class_rec_aux t in
                                                            if List.assoc tit l = None then (String_to_String\<^sub>b\<^sub>a\<^sub>s\<^sub>e tit, body) # l else l in
                                                  case t of
-                                                   OclTy_class obj \<Rightarrow>
+                                                   OclTy_object (OclTyObj (OclTyCore obj) _) \<Rightarrow>
                                                      let t = \<lambda>ty. OclTy_collection (ocl_multiplicity_ext [] None ty ()) (OclTy_class_pre (TyObjN_role_ty (TyObj_to obj))) in
                                                      f (t Sequence) (f (t Set) l)
                                                  | OclTy_collection _ _ \<Rightarrow> f t l
